examples/Yield/Lang.v
@@ -33,6 +33,7 @@ From CTreeYield Require Import
 (*      Events.StateFacts. *)
 
 (* Import Monads. *)
+Import ListNotations.
 Import MonadNotation.
 Local Open Scope monad_scope.
 Local Open Scope string_scope.
@@ -63,21 +64,10 @@ Variant ImpState : Type -> Type :=
 | GetVar (x : var) : ImpState value
 | SetVar (x : var) (v : value) : ImpState unit.
 
-(* Inductive spawn1E (E : Type -> Type) : Type -> Type := *)
-(* | Spawn1 : forall (t : ctree (E +' spawn1E E) unit), spawn1E E unit. *)
-
-(* Inductive spawnE C (E : Type -> Type) : Type -> Type := *)
-(* | Spawn : forall (t: C -> ctree (E +' spawnE C E) (C * unit)), spawnE C E unit. *)
-
 Section Denote1.
+  (* Definition E : Type -> Type := stateE value +' spawnE. *)
 
-
-  (* Context {E' : Type -> Type}. *)
-  (* Context {HasImpState : ImpState -< E'}. *)
-  Definition E : Type -> Type := stateE value +' spawnE.
-  (* Context {HasSpawn1 : spawn1E  -< eff}. *)
-
-  Fixpoint denote_expr (e : expr) : ctree E value :=
+  Fixpoint denote_expr (e : expr) : ctree (stateE value +' spawnE) value :=
     match e with
     | Var v     => trigger (Get _)
     | Lit n     => ret n
@@ -86,12 +76,12 @@ Section Denote1.
     | Mult a b  => l <- denote_expr a ;; r <- denote_expr b ;; ret (l * r)
     end.
 
-  Definition while (step : ctree E (unit + unit)) : ctree E unit :=
+  Definition while (step : ctree (stateE value +' spawnE) (unit + unit)) : ctree (stateE value +' spawnE) unit :=
     CTree.iter (fun _ => step) tt.
 
   Definition is_true (v : value) : bool := if (v =? 0)%nat then false else true.
 
-  Fixpoint denote_imp (s : stmt) : ctree E unit :=
+  Fixpoint denote_imp (s : stmt) : ctree (stateE value +' spawnE) unit :=
     match s with
     | Assign x e =>  v <- denote_expr e ;; trigger (Put _ v)
     | Seq a b    =>  denote_imp a ;; denote_imp b
@@ -110,30 +100,42 @@ Section Denote1.
                                  then (denote_imp t;; ChoiceI 0 (fun _ => ret tt)) (* force the thread to halt here *)
                                  else ret tt)
     | Skip => ret tt
+
+    (* | Atomic t => translate ... (denote_imp t) *)
     end.
 
-  Definition h_state {E} : forall X, stateE value X -> Monads.stateT value (ctree E) X :=
+  Definition h_state {E} `{yieldE value -< E} : forall X, stateE value X -> Monads.stateT value (ctree E) X :=
     fun _ e s =>
       match e with
       | Get _ => Ret (s, s)
       | Put _ s' => Ret (s', tt)
       end.
 
+  Definition h_state_yield {E} `{yieldE value -< E} : forall X, stateE value X -> Monads.stateT value (ctree E) X :=
+    fun _ e s =>
+      match e with
+      | Get _ => s' <- trigger (Yield _ s);; Ret (s', s')
+      | Put _ s' => s'' <- trigger (Yield _ s');; Ret (s'', tt)
+      end.
+
   #[global] Instance MonadChoice_stateT {M S} {MM : Monad M} {AM : Utils.MonadChoice M}
     : Utils.MonadChoice (Monads.stateT S M).
   Admitted.
 
-  Definition handler : forall X, E X -> Monads.stateT value (ctree spawnE) X :=
-    (fun X (e : E X) =>
+  Definition handler : forall X, (stateE value +' spawnE) X -> Monads.stateT value (ctree (parE value)) X :=
+    (fun X (e : (stateE value +' spawnE) X) =>
        match e with
-       | inl1 e' => @h_state spawnE _ e'
+       | inl1 e' => h_state _ e'
        | inr1 e' =>
-         match e' in spawnE R return Monads.stateT value (ctree spawnE) R with
+         match e' in spawnE R return Monads.stateT value (ctree (parE value)) R with
          | Par.Spawn => fun s => b <- trigger Par.Spawn;; Ret(s, b) (* TODO: use MonadTrigger *)
          end
        end).
 
-  Definition interp_state (t : ctree E unit) : Monads.stateT value (ctree spawnE) unit :=
+  Definition interp_state (t : ctree (stateE value +' spawnE) unit) : thread :=
     Interp.interp handler t.
+
+  Definition schedule_denot (t : stmt) : completed :=
+    schedule (interp_state (denote_imp t)) [].
 
 End Denote1.
